new/proof/github_com/goose_lang/goose/model/channel/logatom/chan_au_send.v
@@ -7,39 +7,455 @@ From New.proof.github_com.goose_lang.std Require Import std_core.
 From New.proof.sync_proof Require Import mutex sema.
 
 Section atomic_specs.
-Context `{hG: heapGS Σ, !ffi_semantics _ _}. 
+Context `{hG: heapGS Σ, !ffi_semantics _ _}.
 Context `{!chanGhostStateG Σ V}.
 Context `{!IntoVal V}.
 Context `{!IntoValTyped V t}.
 Context `{!globalsGS Σ} {go_ctx : GoContext}.
 
 Lemma wp_TrySend (ch: loc) (cap: Z) (v: V) (γ: chan_names) (P: iProp Σ):
-  ∀ Φ (b: bool),
+  ∀ Φ,
   is_pkg_init channel ∗ is_channel ch cap γ -∗
-  (* P is here to support helping within a select statement. This is because the internal choice of 
-  which case's atomic update cannot be made prematurely if an offer isn't accepted, so we need to 
-  store the whole collective conjunct of atomic updates in the channel mutex invariant for the 
-  channel we are making an offer on. *)
-  P ∗ (P -∗ ((send_au_fast ch cap v γ (Φ (#true))))) -∗ 
-  (* Keep resources for attempts at this and/or other ops *)
-  (P -∗ (Φ (#false))) -∗ 
+  P ∗ (P -∗ ((send_au_slow ch cap v γ (Φ (#true))))) -∗
+  (P -∗ (Φ (#false))) -∗
   WP ch @ (ptrT.id channel.Channel.id) @ "TrySend" #t #v #true {{ Φ }}.
 Proof.
-Admitted.
+  intros. iIntros "[#Hinit Hunb]". iIntros "[HP HPau]". iIntros "HPfail".
+  try (iModIntro (□ _)%I).
+  let x := ident:(Φ) in
+  try clear x.
+  destruct_pkg_init "Hinit".
+  try (first [ wp_func_call | wp_method_call ]; wp_call; [idtac]).
+  iNamed "Hunb".
+  wp_auto_lc 5.
+  wp_apply (wp_Mutex__Lock with "[$lock]") as "[Hlock Hchan]".
+  iNamed "Hchan".
+
+  (* Case analysis on channel state *)
+  destruct s.
+
+  { (* Buffered channel *)
+    iNamed "phys". iNamed "offer". wp_auto. unfold chan_cap_valid in Hcapvalid.
+    wp_if_destruct.
+    {
+      wp_auto. wp_apply wp_slice_literal. iIntros (sl) "Hsl". wp_auto.
+      iDestruct (own_slice_len with "slice") as "[%Hl %Hcap2]".
+      iDestruct (slice.own_slice_len with "slice") as "[%Hlen_slice %Hslgtz]".
+      iDestruct (own_slice_wf with "slice") as "%Hwf".
+      wp_apply (wp_slice_append with "[$slice $Hsl $slice_cap]").
+      iIntros (fr) "(Hfr & Hfrsl & Hsl)". wp_auto_lc 1.
+      iApply "HPau" in "HP".
+      unfold send_au_slow.
+
+      iApply fupd_wp. iMod "HP".
+      iMod (lc_fupd_elim_later with "[$] HP") as "Hlogatom".
+      iNamed "Hlogatom".
+      iAssert (own_channel ch cap (chan_rep.Buffered buff) γ)%I with "[Hchanrepfrag]" as "Hown".
+      { iFrame. iPureIntro. unfold chan_cap_valid. done. }
+      iDestruct (own_channel_agree with "[$Hown] [$Hoc]") as "%Hseq".
+      subst s.
+
+      iDestruct (own_channel_halves_update _ _ _ _ (chan_rep.Buffered (buff ++ [v]))
+        with "[$Hoc] [$Hown]") as ">[Hgv1 Hgv2]".
+      destruct (length buff <? cap) eqn: Heq.
+      {
+        iMod ("Hcont" with "Hgv1") as "Hstep". iModIntro.
+        wp_apply (wp_Mutex__Unlock with "[$lock state buffer Hfr Hfrsl Hgv2 $Hlock]").
+        { iModIntro. unfold chan_inv_inner. iExists (Buffered (buff ++ [v])). iFrame. }
+        done.
+      }
+      {
+        replace (sint.Z slice_val.(slice.len_f)) with (sint.Z (length buff)) in * by word.
+        word.
+      }
+    }
+    {
+      wp_auto.
+      wp_apply (wp_Mutex__Unlock
+        with "[$lock state slice_cap Hchanrepfrag buffer slice $Hlock]").
+      { iModIntro. unfold chan_inv_inner. iExists (Buffered buff). iFrame.
+        iPureIntro. done.
+      }
+      iApply "HPfail" in "HP". done.
+    }
+  }
+
+  { (* Idle - make offer *)
+    iNamed "phys". wp_auto_lc 5.
+    iNamed "offer".
+    iDestruct ((offer_idle_to_send γ v P (Φ (# true))) with "Hoffer") as ">[offer1 offer2]".
+
+    wp_apply (wp_Mutex__Unlock
+      with "[$lock state v slice slice_cap buffer offer1 Hpred Hchanrepfrag HPau HP $Hlock]").
+    { iModIntro. unfold chan_inv_inner. iExists (SndWait v). iFrame. iPureIntro. done. }
+
+    wp_apply (wp_Mutex__Lock with "[$lock]") as "[Hlock Hchan]".
+    iNamed "Hchan".
+    iNamed "phys". iNamed "offer".
+    destruct s.
+
+    {
+      iNamed "phys". wp_auto_lc 5.
+      unfold chan_cap_valid in Hcapvalid. subst cap.
+      iNamed "offer".
+      unfold chan_cap_valid in Hcapvalid. done.
+    }
+
+    {
+      iNamed "phys". wp_auto_lc 5.
+      iNamed "offer".
+      unfold offer_bundle_empty.
+      iExFalso.
+      iApply (saved_offer_half_full_invalid with "offer2 Hoffer").
+    }
+
+    {
+      unfold chan_phys. iNamed "phys". wp_auto_lc 5.
+      iNamed "offer".
+      iDestruct ((offer_bundle_lc_agree γ (Some (chan_au_base.Snd v)) P (Φ (# true))
+        (Some (chan_au_base.Snd v1)) P0 Φ0)
+        with " [$] [$] [$offer2] [$Hoffer]") as ">(%Heq & Hpeq & H & H1)".
+      iMod ((saved_prop.saved_pred_update (K Φr0)) with "Hpred") as "[Hpred1 Hpred2]".
+      iCombine "Hpred1 Hpred2" as "Hp".
+      wp_apply (wp_Mutex__Unlock
+        with "[$lock state v slice slice_cap buffer Hchanrepfrag Hp H1 $Hlock]").
+      { iModIntro. unfold chan_inv_inner. iExists (Idle). iFrame.
+        iExists Φr0. iFrame. unfold saved_prop.saved_pred_own. rewrite dfrac_op_own Qp.half_half.
+        iFrame.
+        done.
+      }
+      iRewrite -"Hpeq" in "HP".
+      iApply "HPfail" in "HP".
+      done.
+    }
+
+    {
+      iNamed "phys". wp_auto_lc 5.
+      iNamed "offer".
+      iExFalso.
+      iDestruct (offer_bundle_agree with "[$offer2 $Hoffer]") as "[%Heq _]".
+      discriminate Heq.
+    }
+
+    {
+      iNamed "phys". wp_auto_lc 5.
+      iNamed "offer".
+      iExFalso.
+      iDestruct (offer_bundle_agree with "[$offer2 $Hoffer]") as "[%Heq _]".
+      discriminate Heq.
+    }
+
+    {
+      iNamed "phys". wp_auto_lc 5.
+      iNamed "offer".
+
+      unfold send_au_inner.
+      iApply fupd_wp.
+      iMod "Hau".
+      iMod (lc_fupd_elim_later with "[$] Hau") as "HP".
+      iNamed "HP".
+      iAssert (own_channel ch cap (chan_rep.RcvCommit) γ)%I
+        with "[Hchanrepfrag]" as "Hown".
+      { iFrame. iPureIntro. unfold chan_cap_valid. done. }
+      iDestruct (own_channel_agree with "[$Hocinner] [$Hown]") as "%Hseq". subst s.
+      iDestruct (own_channel_halves_update ch cap _ _
+        (chan_rep.Idle)
+        with "[$Hocinner] [$Hown]") as ">[Hgv1 Hgv2]".
+      iMod ("Hcontinner" with "Hgv1") as "Hcont".
+      iModIntro.
+      iDestruct ((offer_bundle_lc_agree γ (Some (chan_au_base.Snd v)) P (Φ (# true))
+        (Some (chan_au_base.Snd v1))
+        P0 Φ0)
+        with " [$] [$] [$offer2] [$Hoffer]") as ">(%Heq & Hpeq & H & H1)".
+
+      wp_apply (wp_Mutex__Unlock
+        with "[$lock state v slice slice_cap buffer Hpred Hgv2 Hpeq H1 $Hlock]").
+      { iModIntro. unfold chan_inv_inner. iExists (Idle). iFrame. }
+      unfold K.
+      iRewrite -"H" in "Hcont". done.
+    }
+
+    {
+      iNamed "phys".
+      unfold chan_logical.
+      destruct draining.
+      {
+        iNamed "phys". iDestruct "offer" as "[Hoc Hoffer]".
+        iNamed "Hoc".
+        unfold chan_cap_valid in *. subst cap. simpl.
+        iNamed "Hoffer". unfold offer_bundle_empty.
+        iDestruct (saved_offer_fractional_invalid with "[$offer2] [$Hoffer]") as "H".
+        { done. }
+        done.
+      }
+      {
+        iNamed "phys". iDestruct "offer" as "[Hoc Hoffer]".
+        iNamed "Hoc".
+        unfold chan_cap_valid in *. subst cap. iNamed "Hoffer". done.
+      }
+    }
+  }
+
+  { (* SndWait *)
+    iNamed "phys". wp_auto_lc 5.
+    wp_apply (wp_Mutex__Unlock
+      with "[$lock state v slice slice_cap buffer offer $Hlock]").
+    { iModIntro. unfold chan_inv_inner. iExists (SndWait v0). iFrame. }
+    iApply "HPfail" in "HP".
+    done.
+  }
+
+  { (* RcvWait - unbuffered channel *)
+    iNamed "phys". wp_auto_lc 2.
+    iNamed "offer". iDestruct "HP" as "HP0". iNamed "offer".
+    iApply "Hau" in "HP".
+    unfold send_au_slow.
+    iApply fupd_wp. iMod "HP".
+    iMod (lc_fupd_elim_later with "[$] HP") as "HP". iNamed "HP".
+    iDestruct "Hoc" as "[H1 H2]".
+    iDestruct (chan_rep_agree with "[$H1] [$Hchanrepfrag]") as "%Hseq". subst s.
+    iAssert (own_channel ch cap (chan_rep.Idle) γ)%I
+      with "[Hchanrepfrag]" as "Hown".
+    { iFrame. iPureIntro. done. }
+    iAssert (own_channel ch cap (chan_rep.Idle) γ)%I
+      with "[H1]" as "Hown1".
+    { iFrame. iPureIntro. done. }
+    iDestruct (own_channel_halves_update ch cap _ _ (chan_rep.RcvPending)
+      with "[$Hown] [$Hown1]") as ">[Hgv1 Hgv2]".
+    iMod ("Hcont" with "Hgv2") as "Hcont1". iModIntro.
+    iApply "HPau" in "HP0".
+    iApply fupd_wp.
+    iMod (lc_fupd_elim_later with "[$] HP0") as "HP0".
+    unfold rcv_au_fast.
+    iMod "HP0".
+    iMod (lc_fupd_elim_later with "[$] HP0") as "HP".
+    iNamed "HP".
+    iDestruct (own_channel_agree with "[$Hgv1] [$Hoc]") as "%Hseq". subst s.
+    iDestruct (own_channel_halves_update _ _ _ _ (chan_rep.SndCommit v)
+      with "[$Hgv1] [$Hoc]") as ">[Hgv1 Hgv2]".
+    iMod ("Hcont" with "Hgv2") as "Hcont". iModIntro.
+    wp_apply (wp_Mutex__Unlock
+      with "[$lock state v slice slice_cap buffer Hgv1 H2 Hpred Hoffer Hcont1 $Hlock]").
+    { iModIntro. unfold chan_inv_inner. iExists (SndDone v). iFrame. iNamed "Hgv1". iFrame. }
+    done.
+  }
+
+  { (* SndDone *)
+    iNamed "phys". wp_auto_lc 2.
+    wp_apply (wp_Mutex__Unlock
+      with "[$lock state v slice slice_cap buffer offer $Hlock]").
+    { iModIntro. unfold chan_inv_inner. iExists (SndDone v0). iFrame. }
+    iApply "HPfail" in "HP". done.
+  }
+
+  { (* RcvDone *)
+    iNamed "phys". wp_auto_lc 2.
+    wp_apply (wp_Mutex__Unlock
+      with "[$lock state v slice slice_cap buffer offer $Hlock]").
+    { iModIntro. unfold chan_inv_inner. iExists (RcvDone v0). iFrame. }
+    iApply "HPfail" in "HP". done.
+  }
+
+  { (* Closed *)
+    destruct draining.
+    {
+      iNamed "phys". iDestruct "offer" as "[Hoc Hoffer]".
+      iNamed "Hoc". iApply "HPau" in "HP".
+      unfold send_au_slow.
+      iApply fupd_wp.
+      iMod "HP".
+      iMod (lc_fupd_elim_later with "[$] HP") as "HP".
+      iNamed "HP".
+      iAssert (own_channel ch cap (chan_rep.Closed []) γ)%I
+        with "[Hchanrepfrag]" as "Hown".
+      { iFrame. }
+      iDestruct (own_channel_agree with "[$Hoc] [$Hown]") as "%Hseq". subst s.
+      done.
+    }
+    {
+      iNamed "phys". iDestruct "offer" as "[Hoc %Hoffer]".
+      iNamed "Hoc". iApply "HPau" in "HP".
+      unfold send_au_slow.
+      iApply fupd_wp.
+      iMod "HP".
+      iMod (lc_fupd_elim_later with "[$] HP") as "HP".
+      iNamed "HP".
+      iAssert (own_channel ch cap (chan_rep.Closed (v0 :: draining)) γ)%I
+        with "[Hchanrepfrag]" as "Hown".
+      { iFrame. iPureIntro. unfold chan_cap_valid. done. }
+      iDestruct (own_channel_agree with "[$Hoc] [$Hown]") as "%Hseq". subst s.
+      done.
+    }
+  }
+Qed.
 
 Lemma wp_TrySend_nb (ch: loc) (cap: Z) (v: V) (γ: chan_names) (P: iProp Σ):
   ∀ Φ,
   is_pkg_init channel ∗ is_channel ch cap γ -∗
-  (* P is here to support helping within a select statement. This is because the internal choice of 
-  which case's atomic update cannot be made prematurely if an offer isn't accepted, so we need to 
-  store the whole collective conjunct of atomic updates in the channel mutex invariant for the 
-  channel we are making an offer on. *)
-  P ∗ (P -∗ ((send_au_slow ch cap v γ (Φ (#true))))) -∗ 
-  (* Keep resources for attempts at this and/or other ops *)
-  (P -∗ (Φ (#false))) -∗ 
+  P ∗ (P -∗ ((send_au_fast ch cap v γ (Φ (#true))))) -∗
+  (P -∗ (Φ (#false))) -∗
   WP ch @ (ptrT.id channel.Channel.id) @ "TrySend" #t #v #false {{ Φ }}.
 Proof.
-Admitted.
+  intros. iIntros "[#Hinit Hunb]". iIntros "[HP HPau]". iIntros "HPfail".
+  try (iModIntro (□ _)%I).
+  let x := ident:(Φ) in
+  try clear x.
+  destruct_pkg_init "Hinit".
+  try (first [ wp_func_call | wp_method_call ]; wp_call; [idtac]).
+  iNamed "Hunb".
+  wp_auto_lc 5.
+  wp_apply (wp_Mutex__Lock with "[$lock]") as "[Hlock Hchan]".
+  iNamed "Hchan".
+
+  (* Case analysis on channel state *)
+  destruct s.
+
+  { (* Buffered channel *)
+    iNamed "phys". iNamed "offer". wp_auto. unfold chan_cap_valid in Hcapvalid.
+    wp_if_destruct.
+    {
+      wp_auto. wp_apply wp_slice_literal. iIntros (sl) "Hsl". wp_auto.
+      iDestruct (own_slice_len with "slice") as "[%Hl %Hcap2]".
+      iDestruct (slice.own_slice_len with "slice") as "[%Hlen_slice %Hslgtz]".
+      iDestruct (own_slice_wf with "slice") as "%Hwf".
+      wp_apply (wp_slice_append with "[$slice $Hsl $slice_cap]").
+      iIntros (fr) "(Hfr & Hfrsl & Hsl)". wp_auto_lc 1.
+      iApply "HPau" in "HP".
+      unfold send_au_slow.
+
+      iApply fupd_wp. iMod "HP".
+      iMod (lc_fupd_elim_later with "[$] HP") as "Hlogatom".
+      iNamed "Hlogatom".
+      iAssert (own_channel ch cap (chan_rep.Buffered buff) γ)%I with "[Hchanrepfrag]" as "Hown".
+      { iFrame. iPureIntro. unfold chan_cap_valid. done. }
+      iDestruct (own_channel_agree with "[$Hown] [$Hoc]") as "%Hseq".
+      subst s.
+
+      iDestruct (own_channel_halves_update _ _ _ _ (chan_rep.Buffered (buff ++ [v]))
+        with "[$Hoc] [$Hown]") as ">[Hgv1 Hgv2]".
+      destruct (length buff <? cap) eqn: Heq.
+      {
+        iMod ("Hcont" with "Hgv1") as "Hstep". iModIntro.
+        wp_apply (wp_Mutex__Unlock with "[$lock state buffer Hfr Hfrsl Hgv2 $Hlock]").
+        { iModIntro. unfold chan_inv_inner. iExists (Buffered (buff ++ [v])). iFrame. }
+        done.
+      }
+      {
+        replace (sint.Z slice_val.(slice.len_f)) with (sint.Z (length buff)) in * by word.
+        word.
+      }
+    }
+    {
+      wp_auto.
+      wp_apply (wp_Mutex__Unlock
+        with "[$lock state slice_cap Hchanrepfrag buffer slice $Hlock]").
+      { iModIntro. unfold chan_inv_inner. iExists (Buffered buff). iFrame.
+        iPureIntro. done.
+      }
+      iApply "HPfail" in "HP". done.
+    }
+  }
+
+  { (* Idle *)
+    iNamed "phys". wp_auto_lc 5.
+    wp_apply (wp_Mutex__Unlock
+      with "[$lock state v slice slice_cap buffer offer HPau $Hlock]").
+    { iModIntro. iFrame. unfold chan_inv_inner. iExists (Idle). iFrame. }
+    iApply "HPfail" in "HP". done.
+  }
+
+  { (* SndWait *)
+    iNamed "phys". wp_auto_lc 5.
+    wp_apply (wp_Mutex__Unlock
+      with "[$lock state v slice slice_cap buffer offer $Hlock]").
+    { iModIntro. unfold chan_inv_inner. iExists (SndWait v0). iFrame. }
+    iApply "HPfail" in "HP".
+    done.
+  }
+
+  { (* RcvWait - unbuffered channel *)
+    iNamed "phys". wp_auto_lc 2.
+    iNamed "offer". iDestruct "HP" as "HP0". iNamed "offer".
+    iApply "Hau" in "HP".
+    unfold send_au_slow.
+    iApply fupd_wp. iMod "HP".
+    iMod (lc_fupd_elim_later with "[$] HP") as "HP". iNamed "HP".
+    iDestruct "Hoc" as "[H1 H2]".
+    iDestruct (chan_rep_agree with "[$H1] [$Hchanrepfrag]") as "%Hseq". subst s.
+    iAssert (own_channel ch cap (chan_rep.Idle) γ)%I
+      with "[Hchanrepfrag]" as "Hown".
+    { iFrame. iPureIntro. done. }
+    iAssert (own_channel ch cap (chan_rep.Idle) γ)%I
+      with "[H1]" as "Hown1".
+    { iFrame. iPureIntro. done. }
+    iDestruct (own_channel_halves_update ch cap _ _ (chan_rep.RcvPending)
+      with "[$Hown] [$Hown1]") as ">[Hgv1 Hgv2]".
+    iMod ("Hcont" with "Hgv2") as "Hcont1". iModIntro.
+    iApply "HPau" in "HP0".
+    iApply fupd_wp.
+    iMod (lc_fupd_elim_later with "[$] HP0") as "HP0".
+    unfold rcv_au_fast.
+    iMod "HP0".
+    iMod (lc_fupd_elim_later with "[$] HP0") as "HP".
+    iNamed "HP".
+    iDestruct (own_channel_agree with "[$Hgv1] [$Hoc]") as "%Hseq". subst s.
+    iDestruct (own_channel_halves_update _ _ _ _ (chan_rep.SndCommit v)
+      with "[$Hgv1] [$Hoc]") as ">[Hgv1 Hgv2]".
+    iMod ("Hcont" with "Hgv2") as "Hcont". iModIntro.
+    wp_apply (wp_Mutex__Unlock
+      with "[$lock state v slice slice_cap buffer Hgv1 H2 Hpred Hoffer Hcont1 $Hlock]").
+    { iModIntro. unfold chan_inv_inner. iExists (SndDone v). iFrame. iNamed "Hgv1". iFrame. }
+    done.
+  }
+
+  { (* SndDone *)
+    iNamed "phys". wp_auto_lc 2.
+    wp_apply (wp_Mutex__Unlock
+      with "[$lock state v slice slice_cap buffer offer $Hlock]").
+    { iModIntro. unfold chan_inv_inner. iExists (SndDone v0). iFrame. }
+    iApply "HPfail" in "HP". done.
+  }
+
+  { (* RcvDone *)
+    iNamed "phys". wp_auto_lc 2.
+    wp_apply (wp_Mutex__Unlock
+      with "[$lock state v slice slice_cap buffer offer $Hlock]").
+    { iModIntro. unfold chan_inv_inner. iExists (RcvDone v0). iFrame. }
+    iApply "HPfail" in "HP". done.
+  }
+
+  { (* Closed *)
+    destruct draining.
+    {
+      iNamed "phys". iDestruct "offer" as "[Hoc Hoffer]".
+      iNamed "Hoc". iApply "HPau" in "HP".
+      unfold send_au_slow.
+      iApply fupd_wp.
+      iMod "HP".
+      iMod (lc_fupd_elim_later with "[$] HP") as "HP".
+      iNamed "HP".
+      iAssert (own_channel ch cap (chan_rep.Closed []) γ)%I
+        with "[Hchanrepfrag]" as "Hown".
+      { iFrame. }
+      iDestruct (own_channel_agree with "[$Hoc] [$Hown]") as "%Hseq". subst s.
+      done.
+    }
+    {
+      iNamed "phys". iDestruct "offer" as "[Hoc %Hoffer]".
+      iNamed "Hoc". iApply "HPau" in "HP".
+      unfold send_au_slow.
+      iApply fupd_wp.
+      iMod "HP".
+      iMod (lc_fupd_elim_later with "[$] HP") as "HP".
+      iNamed "HP".
+      iAssert (own_channel ch cap (chan_rep.Closed (v0 :: draining)) γ)%I
+        with "[Hchanrepfrag]" as "Hown".
+      { iFrame. iPureIntro. unfold chan_cap_valid. done. }
+      iDestruct (own_channel_agree with "[$Hoc] [$Hown]") as "%Hseq". subst s.
+      done.
+    }
+  }
+Qed.
 
 Lemma wp_Send (ch: loc) (cap: Z) (v: V) (γ: chan_names):
   ∀ Φ,
@@ -47,6 +463,252 @@ Lemma wp_Send (ch: loc) (cap: Z) (v: V) (γ: chan_names):
   (send_au_slow ch cap v γ (Φ #())) -∗
   WP ch @ (ptrT.id channel.Channel.id) @ "Send" #t #v {{ Φ }}.
 Proof.
-Admitted.
+  intros. iIntros "[#Hinit #Hic]". iIntros "Hau".
+  try (iModIntro (□ _)%I).
+  iDestruct (is_channel_not_null with "[$Hic]") as "%Hnn".
+  destruct_pkg_init "Hinit".
+  try (first [ wp_func_call | wp_method_call ]; wp_call; [idtac]).
+  wp_auto.
+
+  wp_if_destruct; first done.
+  wp_for. iNamed "Hau".
+  wp_apply ((wp_TrySend ch cap v γ
+    (send_au_slow ch cap v γ (Φ (# ())) ∗ c_ptr ↦ ch ∗ v_ptr ↦ v)%I)
+    with "[][Hau c v]").
+  { iFrame "#". }
+  { iFrame.
+    iIntros "(Hau & c & v)".
+    unfold send_au_slow. iMod "Hau".
+    iModIntro. iModIntro. iNamed "Hau". iFrame.
+    destruct s. all: try done.
+    {
+      destruct (length buff <? cap).
+      {
+        iIntros "H". iMod ("Hcont" with "H") as "H".
+        iModIntro. wp_auto. destruct decide.
+        { wp_auto. wp_for_post. iFrame. naive_solver. }
+        { destruct decide. { wp_auto. done. } done. }
+      }
+      { done. }
+    }
+    {
+      iIntros "H". iMod ("Hcont" with "H") as "H".
+      iModIntro. unfold send_au_inner. iMod "H". iModIntro. iModIntro.
+      iNamed "H".
+      iFrame.
+      destruct s. all: try done.
+      {
+        iIntros "Hcontineer".
+        iMod ("Hcontinner" with "Hcontineer") as "H". iModIntro. wp_auto.
+        destruct decide. all:try naive_solver.
+        destruct decide. all: try done.
+        wp_auto. done.
+      }
+    }
+    {
+      iIntros "Hcontineer".
+      iMod ("Hcont" with "Hcontineer") as "H". iModIntro. wp_auto.
+      destruct decide. all:try naive_solver.
+      destruct decide. all: try done. wp_auto.
+      done.
+    }
+  }
+  {
+    iIntros "Hcontineer". wp_auto.
+    destruct decide. all:try naive_solver.
+    wp_auto. wp_for_post. iFrame.
+  }
+Qed.
+
+Lemma wp_TryClose (ch: loc) (cap: Z) (γ: chan_names) (P: iProp Σ):
+  ∀ Φ,
+  is_pkg_init channel ∗ is_channel ch cap γ -∗
+  P ∗ (P -∗ close_au ch cap γ (Φ (#true))) -∗
+  (P -∗ (Φ (#false))) -∗
+  WP ch @ (ptrT.id channel.Channel.id) @ "TryClose" #t #() {{ Φ }}.
+Proof.
+  intros. iIntros "[#Hinit #Hunb]". iIntros "[HP HPau]". iIntros "HPfail".
+  try (iModIntro (□ _)%I).
+  let x := ident:(Φ) in
+  try clear x.
+  destruct_pkg_init "Hinit".
+  try (first [ wp_func_call | wp_method_call ]; wp_call; [idtac]).
+  iNamed "Hunb".
+  wp_auto_lc 1.
+
+  (* Lock the channel *)
+  wp_apply (wp_Mutex__Lock with "[$lock]") as "[Hlock Hchan]".
+  iNamed "Hchan".
+
+  (* Open the atomic update *)
+  unfold close_au.
+
+  (* Case analysis on channel state *)
+  destruct s; iNamed "phys".
+
+  { (* Buffered *)
+    iNamed "offer".
+    iAssert (own_channel ch cap (chan_rep.Buffered buff) γ)%I
+      with "[Hchanrepfrag]" as "Hown".
+    { iFrame. iPureIntro. done. }
+    wp_auto.
+    iApply fupd_wp. iMod ("HPau" with "HP") as "Hau".
+    iMod (lc_fupd_elim_later with "[$] Hau") as "Hau".
+    iNamed "Hau".
+    iDestruct (own_channel_agree with "[$Hocinner] [$Hown]") as "%Heq".
+    subst s.
+
+    iDestruct (own_channel_halves_update _ _ _ _ (chan_rep.Closed buff)
+      with "[$Hocinner] [$Hown]") as ">[Hgv1 Hgv2]".
+    iMod ("Hcontinner" with "Hgv1") as "HΦ".
+    iModIntro.
+
+    wp_apply (wp_Mutex__Unlock with "[$lock state buffer slice slice_cap Hgv2 $Hlock]").
+    { iModIntro. unfold chan_inv_inner.
+      iExists (Closed buff). unfold chan_phys.
+      destruct buff.
+      { iFrame. destruct cap. all: try iFrame.
+        { simpl. done. }
+        { simpl. done. }
+        { simpl. done. }
+      }
+      { iFrame. }
+    }
+    { iFrame. }
+  }
+
+  { (* Idle *)
+    iNamed "offer".
+    iApply fupd_wp.
+    iMod ("HPau" with "HP") as "Hau".
+    iMod (lc_fupd_elim_later with "[$] Hau") as "Hau".
+    iNamed "Hau".
+    iAssert (own_channel ch cap (chan_rep.Idle) γ)%I
+      with "[Hchanrepfrag]" as "Hown".
+    { iFrame. iPureIntro. done. }
+    iDestruct (own_channel_agree with "[$Hocinner] [$Hown]") as "%Heq".
+    subst s.
+
+    iDestruct (own_channel_halves_update _ _ _ _ (chan_rep.Closed [])
+      with "[$Hocinner] [$Hown]") as ">[Hgv1 Hgv2]".
+    iMod ("Hcontinner" with "Hgv1") as "HΦ".
+    iModIntro.
+
+    wp_auto.
+    wp_apply (wp_Mutex__Unlock with "[$lock state v buffer slice slice_cap Hgv2 Hoffer $Hlock]").
+    { iModIntro. unfold chan_inv_inner.
+      iExists (Closed []). iFrame. destruct cap.
+      { done. }
+      { done. }
+      { done. }
+    }
+    done.
+  }
+
+  { (* SndWait - can't close yet *)
+    wp_auto.
+    wp_apply (wp_Mutex__Unlock with "[$lock state v buffer slice slice_cap offer $Hlock]").
+    { iModIntro. unfold chan_inv_inner. iExists (SndWait v). iFrame. }
+    iApply "HPfail" in "HP". iFrame.
+  }
+
+  { (* RcvWait - can't close yet *)
+    wp_auto.
+    wp_apply (wp_Mutex__Unlock with "[$lock state v buffer slice slice_cap offer $Hlock]").
+    { iModIntro. unfold chan_inv_inner. iExists (RcvWait). iFrame. }
+    iApply "HPfail" in "HP". iFrame.
+  }
+
+  { (* SndDone - can't close yet *)
+    wp_auto.
+    wp_apply (wp_Mutex__Unlock with "[$lock state v buffer slice slice_cap offer $Hlock]").
+    { iModIntro. unfold chan_inv_inner. iExists (SndDone v). iFrame. }
+    iApply "HPfail" in "HP". iFrame.
+  }
+
+  { (* RcvDone - can't close yet *)
+    wp_auto.
+    wp_apply (wp_Mutex__Unlock with "[$lock state v buffer slice slice_cap offer $Hlock]").
+    { iModIntro. unfold chan_inv_inner. iExists (RcvDone v). iFrame. }
+    iApply "HPfail" in "HP". iFrame.
+  }
+
+  { (* Closed - panic case *)
+    iNamed "offer". unfold chan_logical.
+    destruct draining.
+    {
+      iDestruct "offer" as "[offer1 offer2]".
+      iApply fupd_wp.
+      iMod ("HPau" with "HP") as "Hau".
+      iMod (lc_fupd_elim_later with "[$] Hau") as "Hlogatom".
+      iNamed "Hlogatom".
+      iDestruct (own_channel_agree with "[$Hocinner] [$offer1]") as "%Heq".
+      subst s.
+      done.
+    }
+    {
+      iDestruct "offer" as "[offer1 %offer2]".
+      iApply fupd_wp.
+      iMod ("HPau" with "HP") as "Hau".
+      iMod (lc_fupd_elim_later with "[$] Hau") as "Hlogatom".
+      iNamed "Hlogatom".
+      iDestruct (own_channel_agree with "[$Hocinner] [$offer1]") as "%Heq".
+      { iPureIntro. unfold chan_cap_valid. done. }
+      subst s. done.
+    }
+  }
+Qed.
+
+Lemma wp_Close (ch: loc) (cap: Z) (γ: chan_names):
+  ∀ Φ,
+  is_pkg_init channel ∗ is_channel ch cap γ -∗
+  close_au ch cap γ (Φ #()) -∗
+  WP ch @ (ptrT.id channel.Channel.id) @ "Close" #t #() {{ Φ }}.
+Proof.
+  intros. iIntros "[#Hinit #Hic]". iIntros "Hau".
+  try (iModIntro (□ _)%I).
+  iDestruct (is_channel_not_null with "[$Hic]") as "%Hnn".
+  destruct_pkg_init "Hinit".
+  try (first [ wp_func_call | wp_method_call ]; wp_call; [idtac]).
+  wp_auto.
+  simpl.
+  wp_if_destruct; first done.
+  wp_for.
+
+  wp_apply ((wp_TryClose ch cap γ (close_au ch cap γ (Φ (# ())) ∗ c_ptr ↦ ch)%I)
+    with "[$Hic] [Hau c] []").
+  { iFrame. iIntros "[Hau c]".
+    unfold close_au. iMod "Hau". iModIntro. iModIntro. iNamed "Hau". iFrame.
+    destruct s. all: try iFrame.
+    {
+      iIntros "H".
+      iMod ("Hcontinner" with "H") as "H".
+      iModIntro. wp_auto. destruct decide.
+      {
+        wp_auto. wp_for_post. naive_solver.
+      }
+      {
+        destruct decide. all: try done. wp_auto. done.
+      }
+    }
+    {
+      iIntros "H".
+      iMod ("Hcontinner" with "H") as "H".
+      iModIntro. wp_auto. destruct decide.
+      {
+        wp_auto. wp_for_post. naive_solver.
+      }
+      {
+        destruct decide. all: try done. wp_auto. done.
+      }
+    }
+  }
+  iIntros "Hau". iDestruct "Hau" as "[H1 H2]".
+  iApply wp_fupd.
+  wp_auto_lc 1.
+  destruct decide.
+  { iModIntro. wp_auto. wp_for_post. iFrame. }
+  done.
+Qed.
 
 End atomic_specs.
